Test the inline function and applied the correctness

examples/Test.v
@@ -1,12 +1,18 @@
 Require Import Bool String List.
 Require Import Lib.CommonTactics Lib.ilist Lib.Word Lib.Struct Lib.StringBound Lib.FMap.
-Require Import Lts.Syntax Lts.Semantics.
+
+Require Import Lts.Syntax Lts.Semantics Lts.Equiv Lts.Wf.
+Require Import Lts.Inline Lts.InlineFacts_1 Lts.InlineFacts_2.
+Require Import Lts.Decomposition.
 
 Set Implicit Arguments.
 
 Parameter i: nat.
 
-Definition fbCm := MethodSig ("fb"__ i)() : Bool.
+Definition fbCm := MethodSig "fb"() : Bool.
+
+(* Test below after implementing alpha-renaming *)
+(* Definition fbCm := MethodSig ("fb"__ i)() : Bool. *)
 
 Definition ma := MODULE {
   Register "a" : Bool <- Default
@@ -20,14 +26,55 @@ Definition ma := MODULE {
 Definition mb := MODULE {
   Register "b" : Bool <- true
 
-  with Method ("fb"__ i)() : Bool :=
+  with Method "fb"() : Bool :=
     Write "b" <- $$true;
     Read rb <- "b";
     Ret #rb
 }.
 
+Definition mc := MODULE {
+  Register "a" : Bool <- Default
+  with Register "b" : Bool <- true
+
+  with Rule "ra" :=                           
+    Write "b" <- $$true;
+    Read rb : Bool <- "b";
+    Write "a" <- #rb;
+    Retv
+}.
+
 Section Tests.
 
-  Definition mab := ConcatMod ma mb.
+  Definition p : MethsT -> MethsT := id.
+  
+  Lemma mab_mc: traceRefines p (ConcatMod ma mb) mc.
+  Proof.
+    unfold traceRefines; intros.
+    inv H; induction HMultistepBeh.
+
+    - exists (initRegs (getRegInits mc)), nil.
+      split; [|constructor].
+      repeat constructor.
+
+    - apply inline_correct in HStep.
+
+      + simpl in HStep.
+        unfold inlineDmToRule, inlineDmToDm in HStep.
+        simpl in HStep.
+        unfold getBody in HStep.
+        simpl in HStep.
+        destruct (SignatureT_dec _ _); [|elim n0; reflexivity].
+        simpl in HStep.
+        rewrite <-Eqdep.Eq_rect_eq.eq_rect_eq in HStep.
+        unfold appendAction in HStep.
+
+        admit.
+
+      + repeat constructor.
+      + repeat constructor.
+        simpl; auto.
+      + reflexivity.
+
+  Qed.
 
 End Tests.
